\lecture{7}{21 Jan. 10:00}{Functors}
\begin{prev}
	Assume that we initially have a commutative diagram in \(\mathscr{C} \) as
	\[
		\begin{tikzcd}
			X \ar[rd, "g\circ f"']\ar[r, "f"] & Y\ar[d, "g"]\\
			& Z
		\end{tikzcd}
	\]
	After applying \(F\), we'll have
	\[
		\begin{tikzcd}
			F(X) \ar[rd, "F(g\circ f)=F(g)\circ F(f)"']\ar[r, "F(f)"] & F(Y)\ar[d, "F(g)"]\\
			& F(Z)
		\end{tikzcd}
	\]
	which is a commutative diagram in \(\mathscr{D}\).
\end{prev}

We can also have a so-called \underline{contravariant} functor.
\begin{definition}[Contravariant functor]
	Given \(\mathscr{C} , \mathscr{D} \) be two categories. A \underline{contravariant} \emph{functor}
	\[
		F\colon \mathscr{C} \to \mathscr{D}
	\]
	is
	\begin{enumerate}
		\item a map on objects
		      \[
			      \begin{split}
				      F\colon \Object(\mathscr{C} )&\to \Object(\mathscr{D} )\\
				      X&\mapsto F(X).
			      \end{split}
		      \]
		\item maps of morphisms
		      \[
			      \begin{split}
				      \Homomorphism_{\mathscr{C} }(X, Y)&\to \Homomorphism_{\mathscr{D} }(F(Y), F(X))\\
				      \left[f\colon X\to Y\right] &\mapsto \left[F(f)\colon F(Y)\to F(X)\right]
			      \end{split}
		      \]
		      such that
		      \begin{itemize}
			      \item \(F(\identity_{X} ) = \identity_{F(x)} \)
			      \item \(F(f\circ g) = F(g)\circ F(f)\)
		      \end{itemize}
	\end{enumerate}
\end{definition}

Then, we see that in this case, when we apply a contravariant functor \(F\), the diagram becomes
\[
	\begin{tikzcd}
		F(X)  & F(Y)\ar[l, "F(f)"']\\
		& F(Z)\ar[lu, "F(g\circ f)=F(f)\circ F(g)"]\ar[u, "F(g)"']
	\end{tikzcd}
\]
which is a commutative diagram in \(\mathscr{D}\).

\begin{eg}
	Let see some examples.
	\begin{enumerate}
		\item Identity functor.
		      \[
			      I\colon \mathscr{C} \to \mathscr{C}.
		      \]
		\item Forgetful functors.
		      \begin{itemize}
			      \item \[
				            \begin{split}
					            F\colon \underline{\mathrm{Gp}}&\to \underline{\mathrm{set}} \\
					            G&\mapsto G\footnotemark\\
					            \left[f\colon G\to H\right]&\mapsto \left[f\colon G\to H\right]
				            \end{split}
			            \]
			            \addtocounter{footnote}{-1}
			            \stepcounter{footnote}\footnotetext{\(G\) is now just the underlying set of the group \(G\).}
			      \item \[
				            \begin{split}
					            F\colon \underline{\mathrm{Top}}&\to \underline{\mathrm{set}}\\
					            X&\mapsto X\footnotemark\\
					            \left[f\colon X\to Y\right]&\mapsto \left[f\colon X\to Y\right]
				            \end{split}
			            \]
			            \addtocounter{footnote}{-1}
			            \stepcounter{footnote}\footnotetext{\(X\) is now just the underlying set of the topological space \(X\).}
		      \end{itemize}
		\item Free functors.
		      \[
			      \begin{split}
				      \underline{\mathrm{set}}&\to \underline{k\mathrm{-vect}}  \\
				      s&\mapsto \text{"free" \(k\)-vector space on \(s\)}
			      \end{split}
		      \]
		      i.e., vector space with basis \(s\)
		      \[
			      \left[f\colon A\to B\right]\mapsto \left[\text{unique \(k\)-linear map extending \(f\)}\right]
		      \]
		\item
		      \[
			      \begin{split}
				      \underline{k\mathrm{-vect}}&\to \underline{k\mathrm{-vect}}  \\
				      V&\mapsto V^{*} = \Homomorphism _k(V, k)
			      \end{split}
		      \]
		      If we are working in a basis, then we have
		      \[
			      A\mapsto A^{T}.
		      \]
	\end{enumerate}
\end{eg}

\hr

Specifically, we care about two functors.
\begin{enumerate}
	\item
	      \[
		      \begin{split}
			      \underline{\mathrm{Top}^*} &\to \underline{\mathrm{Gp}} \\
			      (X, x_0)&\mapsto \Pi_1(X, x_0)
		      \end{split}
	      \]
	      where \(\Pi _1\) is so-called \emph{fundamental group}.
	\item
	      \[
		      \begin{split}
			      \underline{\mathrm{Top}} &\to \underline{\mathrm{Ab}} \\
			      X&\mapsto \mathrm{Hp}(X)
		      \end{split}
	      \]
	      where \(\mathrm{Hp} \) is so-called \emph{\(p^{th}\) homology}.
\end{enumerate}

Let see the formal definition.

\section{Free Groups}
\begin{definition}[Free group]
	Given a set \(S\), the \emph{free group} is a group \(F_S\) on \(S\) with a map \(S\to F_S\) satisfying the
	universal property.

	If \(G\) is any group, \(f\colon S\to G\) is any map of sets, \(f\) extends uniquely to group homomorphism \(\overline{f} \colon F_S \to G\).
	\[
		\begin{tikzcd}
			S \ar[rd, "f"']\ar[r, ] & F_S\ar[d, dashed, "\exists ! \overline{f} \colon \text{gp hom} "]\\
			& G
		\end{tikzcd}
	\]
\end{definition}
\begin{note}
	This defines a \emph{natural bijection}
	\[
		\Homomorphism_{\underline{\mathrm{set}}}(S, \mathscr{U}(G))\cong \Homomorphism_{\underline{\mathrm{Gp}}}(F_S, G),
	\]
	where \(\mathscr{U} (G)\) is the forgetful functor from the category of groups to the category of sets. This is the
	statement that the free functor and the forgetful functor are \hyperref[def:adjoint-functor]{adjoint};
	specifically that the free functor is the left adjoint (appears on the left in the Hom's above).
\end{note}

\begin{definition}[Adjoints functor]\label{def:adjoint-functor}
	A \underline{free} and \underline{forgetful} functors are \emph{adjoints}.
\end{definition}

\begin{remark}
	Whenever we state a universal property for an object (plus a map), an object (plus a map) \underline{may or may not} exist.
	If such object exists, then it defines the object \textbf{uniquely up to unique isomorphism}, so we can use the universal
	property as the \emph{definition} of the object (plus a map).
\end{remark}

\begin{lemma}
	Universal property defines \(F_S\) (plus a map \(S\to F(S)\) ) uniquely up to unique isomorphism.
\end{lemma}
\begin{proof}
	Fix \(S\). Suppose
	\[
		S\to F_S,\quad S\to \widetilde{F} _S
	\]
	both satisfy the unique property. By universal property, there exist maps such that
	\[
		\begin{tikzcd}
			S \ar[rd, "f"']\ar[r, ] & \widetilde{F}_S\ar[d, dashed, "\exists ! \varphi"]\\
			& F_S
		\end{tikzcd}\qquad
		\begin{tikzcd}
			S \ar[rd, "f"']\ar[r, ] & F_S\ar[d, dashed, "\exists ! \psi"]\\
			& \widetilde{F} _S
		\end{tikzcd}
	\]

	We'll show \(\varphi\) and \(\psi \) are inverses (and the unique isomorphism making above commute). Since
	we must have the following two commutative graphs.
	\[
		\begin{tikzcd}
			& F_S\ar[dd, "\identity_{F_S}"]\\
			S \ar[rd, "f"']\ar[ru, "f"]&\\
			& F_S
		\end{tikzcd}\quad
		\begin{tikzcd}
			& \widetilde{F}_S\ar[dd, "\identity_{\widetilde{F}_S} "]\\
			S \ar[rd, "f"']\ar[ru, "f"]&\\
			& \widetilde{F}_S
		\end{tikzcd}
	\]
	Hence, we see that
	\[
		\begin{tikzcd}
			& F_S\ar[d, "\psi"]\ar[dd, bend left, "\varphi \circ \psi = \identity_{F_S}"]\\
			S \ar[rd, "f"']\ar[ru, "f"]\ar[rd]\ar[r] & \widetilde{F}_S\ar[d, "\varphi"]\\
			& F_S
		\end{tikzcd}\qquad
		\begin{tikzcd}
			& \widetilde{F} _S\ar[d, "\varphi"]\ar[dd, bend left, "\psi \circ \varphi = \identity_{\widetilde{F}_S}"]\\
			S \ar[rd, "f"']\ar[ru, "f"]\ar[rd]\ar[r] & F_S\ar[d, "\psi "]\\
			& \widetilde{F} _S
		\end{tikzcd}
	\]
	where the identity makes these outer triangles commute, then by the uniqueness in universal property, we must have
	\[
		\varphi\circ \psi  = \identity_{F_S},\qquad \psi \circ \varphi = \identity_{\widetilde{F} _S},
	\]
	so \(\varphi\) and \(\psi \) are inverses (thus group isomorphism).
\end{proof}