\lecture{14}{29 Feb.\ 9:30}{Proof of Bahadur's Representation Theorem}
\subsection{Proof of Bahadur's Representation Theorem}
Now we prove the \hyperref[thm:Bahadur-representation]{Bahadur's representation theorem}. Recall the statement.

\begin{prev}
	Given \(F^{\prime} (\theta _p) \eqqcolon f(\theta _p) > 0\) and \(\sqrt{n} (p_n - p) = O(1)\), we want to prove that
	\[
		\sqrt{n} (\hat{\theta} _{p_n} - \theta _p) - \frac{1}{\sqrt{n} } \sum_{i=1}^{n} \frac{p - \mathbbm{1}_{X_i \leq \theta _p} }{f(\theta _p)} - \sqrt{n} \frac{p_n - p}{f(\theta _p)} = o_p(1).
	\]
\end{prev}

We now start the proof.

\begin{proof}[Proof of \autoref{thm:Bahadur-representation}]\label{pf:Bahadur-representation}
	Firstly, we write
	\begin{align*}
		W_n
		 & \coloneqq \sqrt{n} (\hat{\theta} _{p_n} - \theta _p) - \sqrt{n} \frac{p_n - p}{f(\theta _p)} ,          \\
		\shortintertext{and from \(p = F(\theta _p)\),}
		U_n
		 & \coloneqq \frac{1}{\sqrt{n} } \sum_{i=1}^{n} \frac{p - \mathbbm{1}_{X_i \leq \theta _p} }{f(\theta _p)}
		= \frac{\sqrt{n} (p - \hat{F} _n (\theta _p))}{f(\theta _p)}
		= \frac{\sqrt{n} (F(\theta _p) - \hat{F} _n(\theta _p))}{f(\theta _p)},
	\end{align*}
	so we want to show \(W_n - U_n = o_p(1)\). Consider the following lemma.

	\begin{lemma}\label{lma:Bahadur-representation}
		Given two sequences of random variable \((W_n), (U_n)\) such that one of them is \(O_p(1)\) and for every \(\epsilon > 0\) and every \(t \in \mathbb{R} \),
		\[
			\mathbb{P} (W_n \leq t, U_n \geq t+\epsilon ) + \mathbb{P} (U_n \leq t, W_n \geq t + \epsilon ) \to 0,
		\]
		then \(U_n - W_n \overset{p}{\to} 0\).
	\end{lemma}
	\begin{proof}
		Without loss of generality, suppose \(W_n = O_p(1)\), and we show that for every \(\epsilon > 0\), \(\mathbb{P} (\vert W_n - U_n \vert > \epsilon ) \to 0\). Firstly, observe that for every fixed \(\epsilon > 0\), if \(b - a < \epsilon / 2\),
		\[
			\mathbb{P} (a \leq W_n \leq b , \vert W_n - U_n \vert > \epsilon ) \to 0
		\]
		since the left-hand side is equal to
		\[
			\begin{split}
				 & \mathbb{P} (a \leq W_n \leq b, U_n > W_n + \epsilon ) + \mathbb{P} (a \leq W_n \leq b, U_n < W_n - \epsilon ) \\
				 & \leq \mathbb{P} (W_n \leq b, U_n > a + \epsilon ) + \mathbb{P} (a \leq W_n , U_n < b - \epsilon )             \\
				 & \leq \mathbb{P} (W_n \leq b, U_n > a + (2b - 2a) ) + \mathbb{P} (a \leq W_n , U_n < b - (2b - 2a) )           \\
				 & = \mathbb{P} (W_n \leq b, U_n > b + (b - a) ) + \mathbb{P} (a \leq W_n , U_n < a + (a - b) ),
			\end{split}
		\]
		which goes to \(0\) from our assumption. Furthermore, fix any \(\delta > 0\), since \(W_n = O_p(1)\), there exists \(M > 0\) such that \(\mathbb{P} (\vert W_n \vert \leq M) \geq 1 - \delta \) for every \(n \geq 1\). Then,
		\[
			\begin{split}
				\mathbb{P} (\vert U_n - W_n \vert > \epsilon )
				 & \leq \mathbb{P} (\vert W_n \vert > M) + \mathbb{P} (\vert W_n \vert \leq M, \vert U_n - W_n \vert > \epsilon ) \\
				 & \leq \delta + \mathbb{P} (-M \leq W_n \leq M , \vert U_n - W_n \vert > \epsilon ).
			\end{split}
		\]
		The second term is like the first observation, but now we have a larger interval \([-M, M]\) rather than some \([a, b]\) with \(b - a < \epsilon / 2\). To compensate this, consider pair-wise disjoint intervals \((a_i, b_i)\) for \(i \in I\) with \(\vert I \vert < \infty \) such that \(b_i - a_i < \epsilon / 2\) for all \(i \in I\) and \(\bigcup_{i\in I} [a_i, b_i] \supseteq [-M, M]\),
		\[
			\mathbb{P} (-M \leq W_n \leq M , \vert U_n - W_n \vert > \epsilon )
			\leq \sum_{i\in I} \mathbb{P} (a_i \leq W_n \leq b_i, \vert U_n - W_n \vert > \epsilon ).
		\]
		Since \(I\) is finite, together with the first observation, implies \(\limsup_{n \to \infty} \mathbb{P} (\vert U_n - W_n \vert ) \leq \delta\). As \(\delta \) is arbitrary, letting \(\delta \to 0\) completes the proof.
	\end{proof}

	Clearly, \(U_n = O_p(1)\) since it \hyperref[def:converge-in-distribution]{converges in distribution}, so we can try to apply \autoref{lma:Bahadur-representation}. First, we study the numerator of \(U_n\), i.e., \(Z_n(t) \coloneqq \sqrt{n} (F(t) - \hat{F} _n(t))\). We have seen that \(\mathbb{E}_{}[Z_n(t)] = 0\) and \(\Var_{}[Z_n(t)] = F(t) (1 - F(t))\), and \(Z_n(t) \overset{D}{\to} \mathcal{N} (0, F(t) (1 - F(t)))\) by \hyperref[thm:CLT]{central limit theorem}.

	\begin{claim}\label{clm:pf:Bahadur-representation}
		For any \(t, s\in \mathbb{R} \), \(\Var_{}[Z_n(t) - Z_n(s)] = \mathbb{E}_{}[(Z_n(t) - Z_n(s))^2] \leq \vert F(t) - F(s) \vert \). Hence, if \(s_n \to s\) and \(F\) is continuous at \(s\), \(Z_n(s_n) - Z_n(s) \overset{L^2}{\to} 0\), hence \(Z_n(s_n) - Z_n(s) \overset{p}{\to} 0\).
	\end{claim}
	\begin{explanation}
		Observe that \(\Var_{}[Z_n(t) - Z_n(s)] = \Var_{}[\mathbbm{1}_{X \leq t} - \mathbbm{1}_{X \leq s} ] \leq \mathbb{E}_{}[\left\vert \mathbbm{1}_{X \leq t} - \mathbbm{1}_{X \leq s} \right\vert ^2 ]\) where
		\[
			\left\vert \mathbbm{1}_{X \leq t} - \mathbbm{1}_{X \leq s} \right\vert
			= \begin{dcases}
				1, & \text{ if } s < X \leq t \text{ or } t < X \leq s ; \\
				0, & \text{ otherwise} .
			\end{dcases}
		\]
		Hence, as \(\left\vert \mathbbm{1}_{X \leq t} - \mathbbm{1}_{X \leq s} \right\vert = \left\vert \mathbbm{1}_{X \leq t} - \mathbbm{1}_{X \leq s} \right\vert^2\),
		\[
			\begin{split}
				\mathbb{E}_{}[\left\vert \mathbbm{1}_{X \leq t} - \mathbbm{1}_{X \leq s} \right\vert ^2 ]
				 & = \mathbb{P} (s < X \leq t) + \mathbb{P} (t < X \leq s) \\
				 & = (F(t) - F(s))^+ + (F(s) - F(t))^+
				= \vert F(t) - F(s) \vert,
			\end{split}
		\]
		i.e., \(\left\vert \mathbbm{1}_{X \leq t} - \mathbbm{1}_{X \leq s} \right\vert \sim \operatorname{Ber}(\vert F(t) - F(s) \vert ) \).
	\end{explanation}
	From \autoref{lma:Bahadur-representation}, it suffices to show \(\mathbb{P} (W_n \leq t, U_n \geq t + \epsilon ) \to 0\) and \(\mathbb{P} (U_n \leq t , W_n \geq t+\epsilon ) \to 0\) for every \(t \in \mathbb{R} \) and \(\epsilon > 0\). Let's show the first one only. Fix \(t \in \mathbb{R} \) and \(\epsilon > 0\), then
	\begin{align*}
		W_n \leq t
		 & \iff \sqrt{n} (\hat{\theta} _{p_n} - \theta _p) - \sqrt{n} \frac{p_n - p}{f(\theta _p)} \leq t                                                                                                                                                        \\
		 & \iff \hat{\theta} _{p_n} = \hat{F} _n ^{-1} (p_n) \leq \theta _p + \frac{t}{\sqrt{n} } + \frac{p_n - p}{f(\theta _p)} \eqqcolon \theta _p + \delta _n \tag*{\(\displaystyle \delta _n \coloneqq \frac{t}{\sqrt{n} } + \frac{p_n - p}{f(\theta _p)}\)} \\
		\shortintertext{From the property of \(\hat{F} _n ^{-1} \), \(p_n \leq \hat{F} _n(\theta _p + \delta _n)\),}
		 & \iff \sqrt{n} (p_n - F(\theta _p + \delta _n)) \leq \sqrt{n} (\hat{F} _n(\theta _p + \delta _n) - F(\theta _p + \delta _n)) = -Z_n(\theta _p + \delta _n),
	\end{align*}
	which can be written as
	\[
		Z_n(\theta _p + \delta _n) \leq \sqrt{n} (F(\theta _p + \delta _n) - p_n)
		\iff  \frac{Z_n(\theta _p + \delta _n)}{f(\theta _p)} \leq \frac{\sqrt{n} (F(\theta _p + \delta _n) - p_n)}{f(\theta _p)} \eqqcolon t_n .
	\]
	Putting everything together, with \(U_n = Z_n(\theta _p) / f(\theta _p)\), we have
	\[
		\begin{split}
			\mathbb{P} (W_n \leq t, U_n \geq t + \epsilon )
			 & = \mathbb{P} (Z_n(\theta _p + \delta _n) \leq t_n f(\theta _p) , Z_n(\theta _p) \geq f(\theta _p) (t + \epsilon ))        \\
			 & \leq \mathbb{P} (Z_n(\theta _p + \delta _n) - Z_n(\theta _p) \leq (t_n - t - \epsilon ) f(\theta _p))                     \\
			 & = \mathbb{P} \left( \frac{Z_n(\theta _p + \delta _n) - Z_n(\theta _p)}{f(\theta _p)} - (t_n - t) \leq -\epsilon \right) ,
		\end{split}
	\]
	which goes to \(0\) as \(n \to \infty \) if \(t_n \to t\) since from the previous \hyperref[clm:pf:Bahadur-representation]{claim}:
	\begin{itemize}
		\item let \(s_n \coloneqq \theta _p + \delta _n\), \(s \coloneqq \theta _p\), with \(F\) being continuous at \(s\) and \(\delta _n \to 0\), \(Z_n(\theta _p + \delta _n) - Z_n(\theta _p) \overset{p}{\to} 0\);
		\item if further, \(t_n \to t\), the left-hand side goes to \(0\), and the inequality tends to be vacuous.
	\end{itemize}

	\begin{claim}
		Indeed, \(t_n \to t\).
	\end{claim}
	\begin{explanation}
		We want to show that
		\[
			t_n = \frac{F(\theta _p + \delta _n) - p_n}{f(\theta _p) / \sqrt{n} } \to t.
		\]
		By assumption, as \(\delta _n \to 0\) and \(F^{\prime} (\theta _p) = f(\theta _p)\),
		\[
			\frac{F(\theta _p + \delta _n) - F(\theta _p)}{\delta _n} \to f(\theta _p)
			\iff \frac{F(\theta _p + \delta _n) - F(\theta _p) - \delta _n f(\theta _p)}{\delta _n} \to 0,
		\]
		i.e., \(F(\theta _p + \delta _n) = F(\theta _p) + \delta _n f(\theta _p) + o(\delta _n)\). Since \(F(\theta _p) = p\) and \(\delta _n = t / \sqrt{n} + (p_n - p) / f(\theta _p)\),
		\[
			F(\theta _p + \delta _n)
			= p + \left( \frac{t}{\sqrt{n}} + \frac{p_n - p}{f(\theta _p)} \right) f(\theta _p) + o(\delta _n)
			= p + \frac{t}{\sqrt{n} } f(\theta _p) + (p_n - p) + o(\delta _n).
		\]
		Rearranging, with \(o(\delta _n) \cdot \sqrt{n} / f(\theta _p) = \sqrt{n} o(\delta _n) \) from \(f(\theta _p) > 0\), we have
		\[
			t_n
			= \frac{F(\theta _p + \delta _n) - p_n}{f(\theta _p) / \sqrt{n} }
			= t + \sqrt{n} o(\delta _n).
		\]
		Finally, since \(o(\delta _n) = \delta _n o(1)\), with
		\[
			\sqrt{n} \delta _n
			= \sqrt{n} \left( \frac{t}{\sqrt{n} } + \frac{p_n - p}{f(\theta _p)} \right)
			= t + \frac{\sqrt{n} (p_n - p)}{f(\theta _p)}
			= O(1)
		\]
		from our assumption, we have \(\sqrt{n} o(\delta _n) = O(1) o(1) = o(1)\), hence \(t_n = t + o(1) \to t\).
	\end{explanation}
	The second claim \(\mathbb{P} (U_n \leq t, W_n \geq t+\epsilon ) \to 0\) can be proved similarly, hence we're done.
\end{proof}

\section{Inference for Distribution Function}
Since we estimate \(F\) by \(\hat{F} _n\) when estimating \(\theta _p\) by \(\hat{\theta} _p\), one might just as well focus on the former task.

\subsection{Consistency}
Since \(\sqrt{n} (\hat{F} _n(t) - F(t)) \overset{D}{\to} \mathcal{N} (0, F(t) (1 - F(t)))\) for any fixed \(t\), so given \(t_1, \dots , t_m \in \mathbb{R} \), we have
\[
	\begin{pmatrix}
		\sqrt{n} (\hat{F} _n(t_1) - F(t_1)) \\
		\vdots                              \\
		\sqrt{n} (\hat{F} _n(t_m) - F(t_m)) \\
	\end{pmatrix}
	= \begin{pmatrix}
		Z_n(t_1) \\
		\vdots   \\
		Z_n(t_m) \\
	\end{pmatrix}
	= \frac{1}{\sqrt{n} } \sum_{i=1}^{n} \begin{pmatrix}
		\mathbbm{1}_{X_i \leq t_1} - F(t_1) \\
		\vdots                              \\
		\mathbbm{1}_{X_i \leq t_m} - F(t_m) \\
	\end{pmatrix}
	\overset{D}{\to} \mathcal{N} (0, \Sigma )
\]
from \hyperref[thm:multivariate-CLT]{multivariate central limit theorem} where
\[
	\Sigma _{ij} = \Cov_{}[\mathbbm{1}_{X \leq t_i} , \mathbbm{1}_{X \leq t_j} ] = \mathbb{P} (X \leq t_i \land X \leq t_j) - \mathbb{P} (X \leq t_i) \mathbb{P} (X \leq t_j).
\]